ballet/63/examples/archiver/client.e
@@ -1,0 +1,21 @@
+indexing
+	description: "TODO"
+	date: "$Date$"
+	revision: "$Revision$"
+
+class CLIENT
+
+feature
+
+	log (log_file: PROCEDURE [ANY, TUPLE [ANY]]; s: STRING)
+		require
+			log_file_not_void: log_file /= Void
+			s_not_void: s /= Void
+			log_file_valid: log_file.precondition ([s])
+		do
+			log_file.call ([s])
+		ensure
+			log_file_called: log_file.postcondition ([s])
+		end
+
+end
