ballet/63/examples/archiver/tape_archive.e
@@ -1,0 +1,48 @@
+indexing
+	description: "TODO"
+	date: "$Date$"
+	revision: "$Revision$"
+
+class TAPE_ARCHIVE
+
+create
+	make
+
+feature {NONE}
+
+	make
+			-- TODO
+		do
+			create tape
+			is_loaded := tape /= Void
+		ensure
+			tape_not_void: tape /= Void
+			loaded: is_loaded
+		end
+
+feature
+
+	tape: TAPE
+			-- TODO
+
+	is_loaded: BOOLEAN
+			-- TODO
+
+	eject
+		do
+			tape := Void
+			is_loaded := False
+		ensure
+			tape = Void
+			not is_loaded
+		end
+	store (o: ANY)
+			-- TODO
+		require
+			o /= Void
+			is_loaded
+		do
+			tape.save (o)
+		end
+
+end
